src/opt/MemInv.v
@@ -272,9 +272,58 @@ Module MemInv.
       <<SIM2: Memory.sim mem2_tgt mem2_src>>.
   Proof.
     inv PROMISE_TGT.
-    - admit.
-    - admit.
-    - admit.
+    - exploit (@Memory.add_exists mem1_src loc from to val released).
+      { admit. (* m1 sim m2 means m1 and m2 takes the same intervals *) }
+      { inv MEM. inv ADD. auto. }
+      { inv MEM. inv ADD. auto. }
+      i. des.
+      exploit Memory.add_exists_le; try apply LE1_SRC; eauto. i. des.
+      exploit memory_sim_add; try apply SIM1; eauto. i.
+      esplits; eauto.
+      + econs; eauto.
+      + admit. (* inv holds after promises *)
+      + ii. eapply Memory.add_get_inv in LHS; eauto. i. des.
+        * subst. eapply Memory.add_get2. eauto.
+        * apply LE1 in LHS0. eapply Memory.add_get1; eauto.
+    - exploit Memory.split_get0; try apply PROMISES; eauto. i. des.
+      exploit (@Memory.split_exists promises1_src loc from to to2 val released).
+      { apply LE1. eauto. }
+      { inv PROMISES. inv SPLIT. auto. }
+      { inv PROMISES. inv SPLIT. auto. }
+      { inv PROMISES. inv SPLIT. auto. }
+      i. des.
+      exploit Memory.split_exists_le; try apply LE1_SRC; eauto. i. des.
+      exploit memory_sim_split; try apply SIM1; eauto. i.
+      esplits; eauto.
+      + econs; eauto.
+      + admit. (* inv holds after promises *)
+      + ii. eapply Memory.split_get_inv in LHS; eauto. i. des.
+        * subst. eapply Memory.split_get2. eauto.
+        * subst. exploit Memory.split_get1; try apply x1; eauto. i. des; auto.
+          contradict x4. auto.
+        * apply LE1 in LHS1.
+          exploit Memory.split_get1; try apply x1; eauto. i. des; auto.
+          subst. contradict LHS0. auto.
+    - exploit Memory.lower_disjoint; try apply PROMISES; eauto. i.
+      exploit LE1; eauto. i.
+      exploit Memory.lower_exists; eauto.
+      { inv MEM. eauto. }
+      { inv MEM. inv ADD. auto. }
+      { inv MEM. inv ADD. inv ADD0. auto. }
+      i. des.
+      exploit LE1_SRC; eauto. i.
+      exploit Memory.lower_exists; eauto.
+      { inv MEM. eauto. }
+      { inv MEM. inv ADD. auto. }
+      { inv MEM. inv ADD. inv ADD0. auto. }
+      i. des.
+      exploit memory_sim_lower; try apply SIM1; eauto. i.
+      esplits; eauto.
+      + econs; eauto.
+      + admit. (* inv holds after promises *)
+      + ii. eapply Memory.lower_get_inv in LHS; eauto. i. des.
+        * subst. eapply Memory.lower_get2. eauto.
+        * apply LE1 in LHS0. erewrite <- Memory.lower_get1; eauto.
   Admitted.
 
     (* - exploit Memory.add_exists; eauto. i. des. *)
@@ -359,10 +408,40 @@ Module MemInv.
     inv WRITE_TGT. exploit promise; eauto. i. des.
     exploit Memory.promise_lower_promise; try apply PROMISE_SRC; eauto. i. des.
     esplits; eauto.
-    - admit.
-    - admit.
-    - admit.
-    - admit.
+    - admit. (* inv holds after memory operations *)
+    - inv PROMISE; inv PROMISE_SRC.
+      + exploit Memory.add_disjoint; try apply PROMISES0. i.
+        inv INV1. specialize (JOIN loc to).
+        unfold Memory.mem in JOIN. rewrite x1 in JOIN.
+        symmetry in JOIN. apply orb_false_elim in JOIN. des. auto.
+      + exploit Memory.split_disjoint; try apply PROMISES0. i.
+        inv INV1. specialize (JOIN loc to).
+        unfold Memory.mem in JOIN. rewrite x1 in JOIN.
+        symmetry in JOIN. apply orb_false_elim in JOIN. des. auto.
+      + exploit Memory.lower_disjoint; try apply PROMISES. i.
+        inv INV1. specialize (DISJOINT loc to).
+        unfold Memory.mem in DISJOINT. rewrite x1 in DISJOINT.
+        destruct (mem loc to inv); auto. exfalso. apply DISJOINT; auto.
+    - ii. exploit Memory.remove_get_inv; eauto. i. des.
+      inv PROMISE; inv x0.
+      + exploit Memory.add_get_inv; try apply PROMISES; eauto. i. des.
+        { subst. contradict x1. auto. }
+        exploit LE1; eauto. i.
+        exploit Memory.add_get1; try apply PROMISES0; eauto.
+      + exploit Memory.split_get_inv; try apply PROMISES; eauto. i. des; subst.
+        * contradict x1. auto.
+        * exploit Memory.split_get1; try apply PROMISES0; eauto. i. des; auto.
+          contradict x0. auto.
+        * exploit LE1; eauto. i.
+          exploit Memory.split_get1; try apply PROMISES0; eauto. i. des; auto.
+          subst. contradict x3; auto.
+      + exploit Memory.lower_get_inv; try apply PROMISES; eauto. i. des.
+        { subst. contradict x1. auto. }
+        exploit LE1; eauto. i.
+        erewrite <- Memory.lower_get1; eauto.
+    - etrans.
+      + eapply memory_sim_promise; try apply PROMISE_SRC; eauto.
+      + admit. (* promise w/ lower released => sim *)
   Admitted.
 
   Lemma write
